tests/lean/run/premise_selection_mepo.lean
@@ -1,6 +1,6 @@
 import Lean.PremiseSelection.MePo
 
-set_premise_selector fun g _ => Lean.PremiseSelection.mepo (useRarity := false) g
+set_premise_selector Lean.PremiseSelection.mepoSelector (useRarity := false)
 
 example (a b : Int) : a + b = b + a := by
   suggest_premises
@@ -11,7 +11,7 @@ example (x y z : List Int) : x ++ y ++ z = x ++ (y ++ z) := by
   suggest_premises
   sorry
 
-set_premise_selector fun g _ => Lean.PremiseSelection.mepo (useRarity := true) g
+set_premise_selector Lean.PremiseSelection.mepoSelector (useRarity := true)
 
 example (a b : Int) : a + b = b + a := by
   suggest_premises
